examples/l3-machine-code/arm/prog/arm_progScript.sml
@@ -1,5 +1,5 @@
 open HolKernel boolLib bossLib
-open stateLib arm_stepTheory
+open lcsymtacs blastLib stateLib arm_stepTheory
 
 infix \\
 val op \\ = op THEN;
@@ -14,6 +14,8 @@ val _ =
       [["undefined"], ["CurrentCondition"], ["Encoding"]]
       arm_stepTheory.NextStateARM_def
 
+val arm_MEM_def = DB.definition "arm_MEM_def"
+
 val arm_instr_def = Define`
    arm_instr (a, i: word32) =
    { (arm_c_MEM a, arm_d_word8 ((7 >< 0) i));
@@ -23,6 +25,146 @@ val arm_instr_def = Define`
 
 val ARM_IMP_SPEC = Theory.save_thm ("ARM_IMP_SPEC",
    Q.ISPECL [`arm_proj`, `NextStateARM`, `arm_instr`] stateTheory.IMP_SPEC
+   )
+
+(* ------------------------------------------------------------------------ *)
+
+val arm_instr_star = Q.prove(
+   `!a w.
+       {arm_instr (a, w)} =
+       arm_MEM a ((7 >< 0) w) *
+       arm_MEM (a + 1w) ((15 >< 8) w) *
+       arm_MEM (a + 2w) ((23 >< 16) w) *
+       arm_MEM (a + 3w) ((31 >< 24) w)`,
+   srw_tac [wordsLib.WORD_ARITH_EQ_ss]
+       [pred_setTheory.INSERT_UNION_EQ, arm_instr_def, arm_MEM_def,
+        set_sepTheory.STAR_def, set_sepTheory.SPLIT_def]
+   \\ simp [boolTheory.FUN_EQ_THM]
+   \\ metis_tac []
+   )
+
+val arm_instr_star_not_disjoint = Q.prove(
+   `!a w p.
+      ~DISJOINT (arm_instr (a, w)) p ==>
+        ({p} *
+         arm_MEM a ((7 >< 0) w) *
+         arm_MEM (a + 1w) ((15 >< 8) w) *
+         arm_MEM (a + 2w) ((23 >< 16) w) *
+         arm_MEM (a + 3w) ((31 >< 24) w) = SEP_F)`,
+   rw [set_sepTheory.STAR_def, set_sepTheory.SPLIT_def,
+       arm_instr_def, arm_MEM_def, pred_setTheory.DISJOINT_DEF]
+   \\ simp [boolTheory.FUN_EQ_THM, set_sepTheory.SEP_F_def]
+   \\ Cases_on `(arm_c_MEM a,arm_d_word8 ((7 >< 0) w)) IN p`          \\ simp []
+   \\ Cases_on `(arm_c_MEM (a + 1w),arm_d_word8 ((15 >< 8) w)) IN p`  \\ simp []
+   \\ Cases_on `(arm_c_MEM (a + 2w),arm_d_word8 ((23 >< 16) w)) IN p` \\ simp []
+   \\ Cases_on `(arm_c_MEM (a + 3w),arm_d_word8 ((31 >< 24) w)) IN p` \\ simp []
+   \\ fs [pred_setTheory.INSERT_INTER]
+   )
+
+val MOVE_TO_ARM_CODE_POOL = Q.store_thm("MOVE_TO_ARM_CODE_POOL",
+   `!a w c p q.
+       SPEC (STATE arm_proj, NEXT_REL $= NextStateARM, arm_instr, $=)
+        (p *
+         arm_MEM a ((7 >< 0) w) *
+         arm_MEM (a + 1w) ((15 >< 8) w) *
+         arm_MEM (a + 2w) ((23 >< 16) w) *
+         arm_MEM (a + 3w) ((31 >< 24) w))
+        c
+        (q *
+         arm_MEM a ((7 >< 0) w) *
+         arm_MEM (a + 1w) ((15 >< 8) w) *
+         arm_MEM (a + 2w) ((23 >< 16) w) *
+         arm_MEM (a + 3w) ((31 >< 24) w)) =
+       SPEC (STATE arm_proj, NEXT_REL $= NextStateARM, arm_instr, $=)
+        (cond (DISJOINT (arm_instr (a, w)) (BIGUNION (IMAGE arm_instr c))) * p)
+        ((a, w) INSERT c)
+        q`,
+    REPEAT strip_tac
+    \\ once_rewrite_tac [GSYM progTheory.SPEC_CODE]
+    \\ rewrite_tac [stateTheory.CODE_POOL, pred_setTheory.IMAGE_INSERT,
+                    pred_setTheory.IMAGE_EMPTY, pred_setTheory.BIGUNION_INSERT,
+                    pred_setTheory.BIGUNION_EMPTY]
+    \\ Cases_on `DISJOINT (arm_instr (a, w)) (BIGUNION (IMAGE arm_instr c))`
+    \\ rw [stateTheory.UNION_STAR, arm_instr_star, set_sepTheory.SEP_CLAUSES,
+           progTheory.SPEC_FALSE_PRE,
+           AC set_sepTheory.STAR_ASSOC set_sepTheory.STAR_COMM]
+    \\ imp_res_tac arm_instr_star_not_disjoint
+    \\ fs [set_sepTheory.SEP_CLAUSES, progTheory.SPEC_FALSE_PRE,
+           AC set_sepTheory.STAR_ASSOC set_sepTheory.STAR_COMM]
+    )
+
+val sub_intro = Theory.save_thm("sub_intro",
+   simpLib.SIMP_PROVE (srw_ss()) []
+      ``(a + (-b + c) = a - b + c : word32) /\ (a + -b = a - b)``
+   )
+
+val tac = asm_simp_tac (srw_ss()++wordsLib.WORD_CANCEL_ss)
+             [pred_setTheory.INSERT_INTER]
+
+(*
+val top = utilsLib.rhsc (wordsLib.WORD_EVAL_CONV ``word_T - 2w : word32``)
+*)
+
+val DISJOINT_arm_instr = Q.store_thm("DISJOINT_arm_instr",
+   `!a pc x y.
+      3w <+ a /\ a <+ 0xFFFFFFFDw ==>
+      DISJOINT (arm_instr (pc + a, x)) (arm_instr (pc, y))`,
+   rw [arm_instr_def, pred_setTheory.DISJOINT_DEF]
+   \\ `a + 1w <> 0w` by blastLib.FULL_BBLAST_TAC
+   \\ `a + 2w <> 0w` by blastLib.FULL_BBLAST_TAC
+   \\ `a + 3w <> 0w` by blastLib.FULL_BBLAST_TAC
+   \\ `a <> 0w` by blastLib.FULL_BBLAST_TAC
+   \\ `3w <> a` by blastLib.FULL_BBLAST_TAC
+   \\ `2w <> a` by blastLib.FULL_BBLAST_TAC
+   \\ `1w <> a` by blastLib.FULL_BBLAST_TAC
+   \\ tac
+   )
+
+val lem = Q.prove(
+   `!a x y. arm_instr (a + 4w, x) INTER arm_instr (a, y) = {}`,
+   rw [arm_instr_def, pred_setTheory.DISJOINT_DEF]
+   \\ tac
+   )
+
+val DISJOINT_arm_instr_2 = Q.prove(
+   `!a pc x1 x2 y.
+      DISJOINT (arm_instr (pc + a, x1))
+               (arm_instr (pc + a + 4w, x2) UNION arm_instr (pc, y)) =
+      DISJOINT (arm_instr (pc + a, x1)) (arm_instr (pc, y))`,
+   rw [pred_setTheory.DISJOINT_DEF, lem]
+   \\ metis_tac [pred_setTheory.INTER_COMM]
+   )
+
+val rearrange =
+   blastLib.BBLAST_PROVE ``a + (b + c + d) = a + (b + c) + d : word32``
+
+fun disjoint_arm_instr q =
+   DISJOINT_arm_instr
+   |> Q.SPEC q
+   |> Drule.SPEC_ALL
+   |> Conv.CONV_RULE (LAND_CONV blastLib.BBLAST_CONV)
+   |> REWRITE_RULE [rearrange]
+   |> Drule.GEN_ALL
+
+fun disjoint_arm_instr_2 q =
+   DISJOINT_arm_instr_2
+   |> Q.SPEC q
+   |> REWRITE_RULE [sub_intro, wordsTheory.WORD_ADD_ASSOC,
+                    GSYM wordsTheory.WORD_ADD_SUB_ASSOC]
+   |> Drule.GEN_ALL
+
+val disjoint_arm_instr_thms = Theory.save_thm("disjoint_arm_instr_thms",
+   Drule.LIST_CONJ
+     ([disjoint_arm_instr `(w2w (w: word8) + 8w) + 4w`,
+       disjoint_arm_instr `w2w (w: word8) + 8w`,
+       disjoint_arm_instr `w2w (w: word12) + 8w`,
+       disjoint_arm_instr
+         `^(bitstringSyntax.mk_v2w (bitstringSyntax.mk_bstring 10 0, ``:32``))
+          + 8w`,
+       disjoint_arm_instr
+         `(^(bitstringSyntax.mk_v2w (bitstringSyntax.mk_bstring 10 0, ``:32``))
+           + 8w) + 4w`] @
+      List.map disjoint_arm_instr_2 [`a`, `-a`, `a + b`, `a - b`])
    )
 
 (* ------------------------------------------------------------------------ *)
